bin/main.ml
@@ -14,22 +14,18 @@ let typed_module_of_file f =
   let m = module_of_file f in
   Vera.Typecheck.tc_vmodule m
 
-let sort_module_items m =
-  let open Vera in
-  let open Vera.Verilog in
-  let inputs = module_inputs m in
-  match Sort.sort_module_items inputs m.modBody with
-  | None -> Inl (Util.string_to_lst "Sorting failed")
-  | Some modBody -> Inr { m with modBody }
-
 let sorted_module_of_file f =
   let* m = typed_module_of_file f in
-  sort_module_items m
+  Vera.sort_vmodule m
+
+let simpl_module_of_file f =
+  let* m = typed_module_of_file f in
+  Inr (Vera.simpl_vmodule m)
 
 let smt_of_file filename =
   (* Need to tag it as left or right, doesn't matter here because we only
       translate one module *)
-  Vera.verilog_to_smt VerilogLeft =<< sorted_module_of_file filename
+  Vera.verilog_to_smt VerilogLeft =<< simpl_module_of_file filename
 
 let compare ~solver ~dump_query filename1 filename2 =
   let query_result =
@@ -77,6 +73,8 @@ let rec lower level filename =
       display_or_error VerilogPP.Typed.vmodule (typed_module_of_file filename)
   | `Sorted ->
       display_or_error VerilogPP.Typed.vmodule (sorted_module_of_file filename)
+  | `Simplified ->
+      display_or_error VerilogPP.Typed.vmodule (simpl_module_of_file filename)
   | `SMT -> display_or_error SMTPP.SMTLib.query (smt_of_file filename)
   | `All ->
       printf "\n-- parsed -- \n";
