vera/VerilogToSMT/VerilogToSMT.v
@@ -206,24 +206,26 @@ Definition assert_permutation {A} `{forall (x y : A), DecProp (x = y)}
   end.
 
 Definition verilog_to_smt (name_tag : VarTag) (vmodule : Verilog.vmodule) : transf SMTQueries.query :=
-  assert_dec
-    (disjoint (Verilog.module_inputs vmodule) (Verilog.module_outputs vmodule))
-    "Overlapping inputs and outputs"%string ;;
-  assert_dec
-    (NoDup (Verilog.module_body_writes (Verilog.modBody vmodule)))
-    "Duplicate writes"%string ;;
-  let* nodup := assert_dec
-    (NoDup (Verilog.modVariables vmodule))
-    "Duplicate variables"%string in
-  trace "Check for undriven"
-    opt_to_sum "Undriven variables"%string
-      (assert_permutation
-        (Verilog.modVariables vmodule)
-        (Verilog.module_body_writes (Verilog.modBody vmodule) ++ Verilog.module_inputs vmodule)
-	nodup) ;;
-  trace "Check sort" 
-    (assert_dec
-      (module_items_sorted (Verilog.module_inputs vmodule) (Verilog.modBody vmodule))
-      "Module items unsorted"%string);;
-  trace "Convert to SMT" (transfer_module_body name_tag (Verilog.modBody vmodule))
+  trace ("To SMT " ++ Verilog.modName vmodule) (
+    assert_dec
+      (disjoint (Verilog.module_inputs vmodule) (Verilog.module_outputs vmodule))
+      "Overlapping inputs and outputs"%string ;;
+    assert_dec
+      (NoDup (Verilog.module_body_writes (Verilog.modBody vmodule)))
+      "Duplicate writes"%string ;;
+    let* nodup := assert_dec
+      (NoDup (Verilog.modVariables vmodule))
+      "Duplicate variables"%string in
+    trace "Check for undriven"
+      opt_to_sum "Undriven variables"%string
+        (assert_permutation
+          (Verilog.modVariables vmodule)
+          (Verilog.module_body_writes (Verilog.modBody vmodule) ++ Verilog.module_inputs vmodule)
+    	nodup) ;;
+    trace "Check sort" 
+      (assert_dec
+        (module_items_sorted (Verilog.module_inputs vmodule) (Verilog.modBody vmodule))
+        "Module items unsorted"%string);;
+    trace "Convert to SMT" (transfer_module_body name_tag (Verilog.modBody vmodule))
+  )
 .
